WIP: more split counter

split_counter.v
@@ -29,32 +29,68 @@ Definition read :=
 
 Class SplitIG Σ := splitIG {
    split_inG :> inG Σ (authUR (gmapUR nat (exclR (leibnizC (gname * nat)))));
+   split_monotone_inG :> inG Σ (authUR (mnatUR));
 }.
 
 Definition splitΣ :=
-  #[GFunctor (authUR (gmapUR nat (exclR (leibnizC (gname * nat)))))].
+  #[GFunctor (authUR (gmapUR nat (exclR (leibnizC (gname * nat)))));
+      GFunctor (authUR (mnatUR))].
 
-Global Instance subG_splitΣ Σ :
-  subG splitΣ Σ → inG Σ (authUR (gmapUR nat (exclR (leibnizC (gname * nat))))).
+Global Instance subG_splitΣ Σ : subG splitΣ Σ → SplitIG Σ.
 Proof. solve_inG. Qed.
 
 Section counter.
   Context `{SplitIG Σ, heapIG Σ, savedPredG Σ nat}.
 
+  Implicit Types split_name : (gname * gname).
+
   Fixpoint of_Readers_rec (M : list (gname * nat)) i :
     gmap nat (excl (leibnizC (gname * nat))) :=
     match M with
     | [] => ∅
-    | r :: M' => <[i := Excl r]>(of_Readers_rec M' (S i))
+    | r :: M' => {[i := Excl r]} ⋅ (of_Readers_rec M' (S i))
     end.
+
+  Lemma of_Readers_dom M i n : n ∈ dom (gset _) (of_Readers_rec M i) → i ≤ n.
+  Proof.
+    revert i; induction M => i;
+    rewrite /= ?dom_empty; first done.
+    rewrite dom_op elem_of_union dom_singleton elem_of_singleton.
+    intros [Hn|Hn]; subst; auto.
+    cut (S i ≤ n); first omega; auto.
+  Qed.
+
+  Lemma of_Readers_dom' M i n :
+    n ∈ dom (gset _) (of_Readers_rec M i) → n < i + length M.
+  Proof.
+    revert i; induction M => i;
+    rewrite /= ?dom_empty; first done.
+    rewrite dom_op elem_of_union dom_singleton elem_of_singleton.
+    intros [Hn|Hn]; subst; auto with omega.
+    cut (n < S i + length M); first omega; auto.
+  Qed.
+
+  Lemma of_Readers_app M N i :
+    of_Readers_rec (M ++ N) i = (of_Readers_rec N (i + length M)) ⋅ (of_Readers_rec M i).
+  Proof.
+    revert N i.
+    induction M => N i.
+    - by rewrite /= right_id_L; replace (i + 0) with i by omega.
+    - rewrite /= IHM. replace (S i + length M) with (i + S (length M)) by omega.
+      rewrite !assoc_L. f_equal. rewrite (comm_L op) //.
+  Qed.
 
   Definition of_Readers M := of_Readers_rec M 0.
 
-  Definition ownReaders split_name M := own split_name (● (of_Readers M)).
+  Definition ownReaders split_name M := own split_name.1 (● (of_Readers M)).
 
-  Definition ownReader split_name i γ n := own split_name (◯ {[i := Excl (γ, n)]}).
+  Definition ownReader split_name i γ n := own split_name.1 (◯ {[i := Excl (γ, n)]}).
 
   Definition counterN := nroot .@ "counter".
+
+  Definition fullRight split_name n := own split_name.2 (● n).
+
+  Definition fragRight split_name n := own split_name.2 (◯ n).
 
   Definition except_counterN := ⊤ ∖ nclose counterN.
   Lemma except_counterN_eq : except_counterN = ⊤ ∖ nclose counterN.
@@ -70,8 +106,8 @@ Section counter.
            I (snd r) ={except_counterN}=∗ ψ (snd r) ∗ I (snd r))%I.
 
   Definition CounterInv split_name l r I :=
-    (∃ lv rv M, l ↦ (NatV lv) ∗ r ↦ (NatV rv) ∗ I (lv + rv)
-                  ∗ ownReaders split_name M
+    (∃ lv (rv : mnatUR) M, l ↦ (NatV lv) ∗ r ↦ (NatV rv) ∗ fullRight split_name rv ∗
+                  I (lv + rv) ∗ ownReaders split_name M
                   ∗ [∗ list] r ∈ M, reader_inv r (lv + rv) I)%I.
 
   Definition Counter split_name (c : val) (I : nat → iProp Σ) : iProp Σ:=
@@ -89,8 +125,9 @@ Section counter.
     iApply wp_alloc; auto.
     iNext. iIntros (r) "Hr".
     iMod (own_alloc (A := authUR (gmapUR nat (exclR (leibnizC (gname * nat))))) (● ∅))
-      as (split_name) "He"; first done.
-    iMod (inv_alloc counterN _ (CounterInv split_name l r I) with "[-HF]") as "HI".
+      as (γ1) "He"; first done.
+    iMod (own_alloc (A := authUR mnatUR) (● 0)) as (γ2) "He'"; first done.
+    iMod (inv_alloc counterN _ (CounterInv (γ1, γ2) l r I) with "[-HF]") as "HI".
     { iExists _, _, []; rewrite /ownReaders /=; iFrame. }
     iApply wp_value.
     iApply "HF". iExists _, _; eauto.
@@ -120,7 +157,7 @@ Section counter.
     iApply wp_pure_step_later; auto. iNext.
     iApply wp_value; simpl.
     clear rv M.
-    iInv counterN as (lv' rv M) "(Hl & Hr & HI & HM & Hri)" "Hcl".
+    iInv counterN as (lv' rv M) "(Hl & Hr & Hrv & HI & HM & Hri)" "Hcl".
     destruct (decide (lv = lv')); first subst.
     - iApply (wp_cas_suc with "Hl"); iNext; iIntros "Hl".
       iAssert (I (lv' + rv) ={⊤ ∖ ↑counterN}=∗ I (lv' + rv) ∗
@@ -138,17 +175,74 @@ Section counter.
       iMod ("Hri'" with "HI") as "[HI Hri]".
       rewrite !except_counterN_eq.
       iMod ("Hvs" with "HI") as "[HI HQ]".
-      iMod ("Hcl" with "[Hl Hr HI HM Hri]") as "_".
+      iMod ("Hcl" with "[Hl Hr Hrv HI HM Hri]") as "_".
       { replace (lv' + rv + 1) with (lv' + 1 + rv) by omega.
         iNext; iExists _, _, _; iFrame. }
       iModIntro.
       iApply wp_pure_step_later; auto. iNext.
       by iApply wp_value; iApply "HF".
     - iApply (wp_cas_fail with "Hl"); first congruence; iNext; iIntros "Hl".
-      iMod ("Hcl" with "[Hl Hr HI HM Hri]") as "_".
+      iMod ("Hcl" with "[Hl Hr Hrv HI HM Hri]") as "_".
       { iNext; iExists _, _, _; iFrame. }
       iModIntro.
       iApply wp_pure_step_later; auto. iNext.
       iApply ("IH" with "Hvs"); eauto.
   Qed.
 
+  Theorem wp_read split_name c I ψ :
+    {{{Counter split_name c I ∗ ∀ v, I v ={except_counterN}=∗ ψ v ∗ I v}}}
+      App read (of_val c)
+    {{{v, RET (NatV v); ψ v}}}.
+  Proof.
+    iIntros (F) "[#HInv Hvs] HF". iDestruct "HInv" as (l r ->) "HInv".
+    iApply wp_pure_step_later; auto. iNext. asimpl.
+    iApply (wp_bind (fill [LetInCtx _])); simpl.
+    iApply (wp_create_pr _ (λ μ, ∃ n, Shead μ = (NatV n))); trivial.
+    { by exists (Sconst (NatV 0)), 0. }
+    iNext; iIntros (p). iDestruct 1 as (μ) "Hμ".
+    iDestruct (cpvar_contains with "Hμ") as %[n Hμ].
+    iApply wp_pure_step_later; auto. iNext. asimpl.
+    iApply (wp_bind (fill [LetInCtx _])); simpl.
+    iApply (wp_bind (fill [LoadCtx])); simpl.
+    iApply wp_pure_step_later; auto. iNext.
+    iApply wp_value; simpl.
+    iInv counterN as (lv rv M) "(Hl & Hr & Hrv & HI & HM & Hri)" "Hcl".
+    iApply (wp_load with "Hl"). iNext. iIntros "Hl".
+    iMod (saved_pred_alloc ψ) as (γ) "#Hψ".
+    iMod (@own_update _ _ _ _ _ (● (of_Readers (M ++ [(γ, lv + max n rv)])) ⋅
+                                   ◯ ({[length M := Excl (γ, lv + max n rv)]}))
+            with "HM") as "HM".
+    { rewrite /of_Readers of_Readers_app /= right_id_L.
+      apply auth_update_alloc.
+      rewrite -insert_singleton_op; last first.
+      - eapply (not_elem_of_dom (D := gset _)).
+        intros ?%of_Readers_dom'; omega.
+      - apply: alloc_singleton_local_update; last done.
+        eapply (not_elem_of_dom (D := gset _)).
+        intros ?%of_Readers_dom'; omega. }
+    iDestruct "HM" as "[HM Hreader]".
+    iAssert (reader_inv (γ, lv + max n rv) (lv + rv) I)%I with "[Hvs]" as "Hrinv".
+    { rewrite /reader_inv /=; destruct decide; try lia.
+      iExists _; iFrame "#". iApply "Hvs". }
+    iMod (@own_update _ _ _ _ _ (● rv ⋅ ◯ rv) with "Hrv") as "Hrv".
+    { apply (auth_update_alloc).
+      cut ((rv, ε) ~l~> (max rv rv, max rv ε));
+        first replace (max rv rv) with rv by (by rewrite Nat.max_id);
+        first replace (max rv ε) with rv by (by rewrite PeanoNat.Nat.max_0_r);
+        trivial.
+      apply (@op_local_update mnatUR) => ?. admit. }
+    iDestruct "Hrv" as "[Hrv Hrvfrag]".
+    iMod ("Hcl" with "[Hl Hr Hrv HI HM Hri Hrinv]") as "_".
+    { by iNext; iExists _, _, (M ++ [_]); iFrame. }
+    iModIntro.
+    iApply wp_pure_step_later; auto. iNext.
+    iApply (wp_bind (fill [LetInCtx _])); simpl.
+    iApply (wp_bind (fill [LoadCtx])); simpl.
+    iApply wp_pure_step_later; auto. iNext.
+    iApply wp_value; simpl.
+    iInv counterN as (lv' rv' M') "(Hl & Hr & Hrv & HI & HM & Hri)" "Hcl".
+    iApply (wp_load with "Hr"). iNext. iIntros "Hr".
+    iDestruct (own_valid_2 with "Hrvfrag Hrv") as
+        %[Hrv%mnat_included _]%auth_valid_discrete; simpl in *.
+    rewrite -> right_id_L in Hrv; last typeclasses eauto.
+    
